Indexing_Hoare.thy
@@ -1,0 +1,355 @@
+(*
+ * Copyright 2019, NTU
+ *
+ * This software may be distributed and modified according to the terms of
+ * the BSD 2-Clause license. Note that NO WARRANTY is provided.
+ * See "LICENSE_BSD2.txt" for details.
+ *
+ *  Author: Albert Rizaldi, NTU Singapore
+ *)
+
+theory Indexing_Hoare
+  imports VHDL_Hoare_Complete
+begin
+
+datatype sig = IN | OUT
+
+definition index :: "sig conc_stmt" where
+  "index \<equiv> process {IN} : Bassign_trans OUT (Bindex IN 3) 1"
+
+abbreviation "bof_wline tw sig n \<equiv> bval_of (wline_of tw sig n)"
+abbreviation "lof_wline tw sig n \<equiv> lval_of (wline_of tw sig n)"
+
+definition inv :: "sig assn2" where
+  "inv tw \<equiv> (\<forall>i < fst tw. bof_wline tw OUT (i + 1) = (lof_wline tw IN i) ! 3)"
+
+definition inv' :: "sig assn2" where
+  "inv' tw = (disjnt {IN} (event_of tw) \<longrightarrow> (\<forall>i\<ge>fst tw. bof_wline tw OUT (i + 1) = (lof_wline tw IN (fst tw)) ! 3))"
+
+lemma potential_tyenv:
+  assumes "seq_wt \<Gamma> (Bassign_trans OUT (Bindex IN 3) 1)"
+  shows   "\<exists>len>3. \<Gamma> IN = Lty len \<and> \<Gamma> OUT = Bty"
+proof (rule seq_wt_cases(4)[OF assms])
+  assume "bexp_wt \<Gamma> (Bindex IN 3) (\<Gamma> OUT)"
+  then obtain len where "bexp_wt \<Gamma> (Bsig IN) (Lty len) \<and> 3 < len \<and> \<Gamma> OUT = Bty"
+    by (meson bexp_wt_cases(10))
+  hence "\<Gamma> IN = Lty len" and "\<Gamma> OUT = Bty" and "3 < len"
+    by (metis bexp_wt_cases(9))+
+  thus ?thesis
+    by blast
+qed
+
+lemma inv_next_time:
+  assumes "inv tw"
+  assumes "beval_world_raw2 tw (Bindex IN 3) x" and "type_of x = Bty"
+  defines "tw' \<equiv> tw[OUT, 1 :=\<^sub>2 x]"
+  shows   "inv (next_time_world tw', snd tw')"
+  unfolding inv_def
+proof (rule, rule)
+  have "fst tw' < next_time_world tw'"
+    using next_time_world_at_least  using nat_less_le by blast
+  moreover have "fst tw = fst tw'"
+    unfolding tw'_def worldline_upd2_def worldline_upd_def by auto
+  ultimately have "fst tw < next_time_world tw'"
+    by auto
+  fix i
+  assume "i < fst (next_time_world tw', snd tw')"
+  hence "i < next_time_world tw'"
+    by auto
+  hence "i < fst tw \<or> fst tw \<le> i \<and> i < next_time_world tw' - 1 \<or> i = next_time_world tw' - 1"
+    by linarith
+  moreover
+  { assume "i < fst tw"
+    hence "wline_of tw' OUT (i + 1) = wline_of tw OUT (i + 1)"
+      unfolding tw'_def worldline_upd2_def worldline_upd_def by auto
+    hence "bof_wline (next_time_world tw', snd tw') OUT (i + 1) =  bof_wline tw OUT (i + 1)"
+      by simp
+    also have "... = (lof_wline tw IN i) ! 3"
+      using assms(1) \<open>i < fst tw\<close> unfolding inv_def by auto
+    also have "... = (lof_wline (next_time_world tw', snd tw') IN i) ! 3"
+      unfolding tw'_def worldline_upd2_def worldline_upd_def by auto
+    finally have "bof_wline (next_time_world tw', snd tw') OUT (i + 1) =
+                 (lof_wline (next_time_world tw', snd tw') IN i) ! 3"
+      by auto }
+  moreover
+  { assume "fst tw \<le> i \<and> i < next_time_world tw' - 1"
+    hence "bof_wline tw' OUT (i + 1) = bof_wline tw' OUT (fst tw + 1)"
+      using unchanged_until_next_time_world
+      by (metis (no_types, lifting) One_nat_def Suc_lessI Suc_less_eq \<open>get_time tw < next_time_world
+      tw'\<close> \<open>get_time tw = get_time tw'\<close> add.right_neutral add_Suc_right le_SucI le_add1
+      less_diff_conv not_le)
+    also have "... = bval_of x"
+      using assms(4)  by (metis worldline_upd2_at_dly)
+    also have "... = lof_wline tw IN (fst tw) ! 3"
+    proof -
+      have assm2: "beval_world_raw (snd tw) (fst tw) (Bindex IN 3) x"
+        using assms(2) unfolding beval_world_raw2_def by auto
+      have "\<not> is_Bv (wline_of tw IN (fst tw))"
+        apply (rule beval_world_raw_cases[OF assm2], erule beval_cases)
+        by (metis beval_cases(1) comp_apply state_of_world_def val.disc(2))
+      hence "state_of_world (snd tw) (fst tw) IN = Lv (lof_wline tw IN (fst tw))"
+        unfolding state_of_world_def by simp
+      show ?thesis
+        apply (rule beval_world_raw_cases[OF assm2])
+        apply (erule beval_cases)+
+        using \<open>state_of_world (snd tw) (fst tw) IN = Lv (lof_wline tw IN (fst tw))\<close> by simp
+    qed
+    also have "... = lof_wline (next_time_world tw', snd tw') IN i ! 3"
+      by (metis \<open>get_time tw = get_time tw'\<close> \<open>get_time tw \<le> i \<and> i < next_time_world tw' - 1\<close> \<open>i <
+      next_time_world tw'\<close> less_add_one o_apply snd_conv tw'_def unchanged_until_next_time_world
+      worldline_upd2_before_dly)
+    finally have "bof_wline (next_time_world tw', snd tw') OUT (i + 1) =
+                 (lof_wline (next_time_world tw', snd tw') IN i) ! 3"
+      by auto }
+  moreover
+  { assume "i = next_time_world tw' - 1"
+    hence "bof_wline tw' OUT (i + 1) = bof_wline tw' OUT (next_time_world tw')"
+      using \<open>get_time tw < next_time_world tw'\<close> by auto
+    also have "... = bof_wline tw' OUT (fst tw' + 1)"
+      by (smt \<open>get_time tw < next_time_world tw'\<close> \<open>get_time tw = get_time tw'\<close> comp_apply discrete
+      leD snd_conv tw'_def worldline_upd2_at_dly worldline_upd2_def worldline_upd_def)
+    also have "... = bof_wline tw' OUT (fst tw + 1)"
+      by (simp add: \<open>get_time tw = get_time tw'\<close>)
+    also have "... = bval_of x"
+      using assms(4)  by (metis worldline_upd2_at_dly)
+    also have "... = lof_wline tw IN (fst tw) ! 3"
+    proof -
+      have assm2: "beval_world_raw (snd tw) (fst tw) (Bindex IN 3) x"
+        using assms(2) unfolding beval_world_raw2_def by auto
+      have "\<not> is_Bv (wline_of tw IN (fst tw))"
+        apply (rule beval_world_raw_cases[OF assm2], erule beval_cases)
+        by (metis beval_cases(1) comp_apply state_of_world_def val.disc(2))
+      hence "state_of_world (snd tw) (fst tw) IN = Lv (lof_wline tw IN (fst tw))"
+        unfolding state_of_world_def by simp
+      show ?thesis
+        apply (rule beval_world_raw_cases[OF assm2])
+        apply (erule beval_cases)+
+        using \<open>state_of_world (snd tw) (fst tw) IN = Lv (lof_wline tw IN (fst tw))\<close> by simp
+    qed
+    also have "... = lof_wline (next_time_world tw', snd tw') IN i ! 3"
+      by (metis (mono_tags, lifting) \<open>get_time tw < next_time_world tw'\<close> \<open>get_time tw = get_time
+      tw'\<close> \<open>i < next_time_world tw'\<close> \<open>i = next_time_world tw' - 1\<close> add_le_imp_le_diff comp_apply
+      discrete less_add_one snd_conv tw'_def unchanged_until_next_time_world
+      worldline_upd2_before_dly)
+    finally have "bof_wline (next_time_world tw', snd tw') OUT (i + 1) =
+                 (lof_wline (next_time_world tw', snd tw') IN i) ! 3"
+      by auto }
+  ultimately show "bof_wline (next_time_world tw', snd tw') OUT (i + 1) = lof_wline (next_time_world tw', snd tw') IN i ! 3"
+    by auto
+qed
+
+lemma type_correctness_length:
+  assumes "seq_wt \<Gamma> (Bassign_trans OUT (Bindex IN 3) 1)"
+  assumes "wityping \<Gamma> (snd tw)"
+  assumes "beval_world_raw2 tw (Bindex IN 3) x"
+  shows   "type_of x = Bty"
+proof -
+  obtain len where "\<Gamma> IN = Lty len" and "3 < len"
+    using potential_tyenv[OF assms(1)] by auto
+  have *: "beval_world_raw (snd tw) (fst tw) (Bindex IN 3) x"
+    using assms(3) unfolding beval_world_raw2_def by auto
+  have "type_of (state_of_world (snd tw) (fst tw) IN) = Lty len"
+    using assms(2) unfolding wityping_def
+    by (simp add: \<open>\<Gamma> IN = Lty len\<close> state_of_world_def wtyping_def)
+  hence **: "\<And>bs. state_of_world (snd tw) (fst tw) IN = Lv bs \<Longrightarrow> length bs = len"
+    by simp
+  show ?thesis
+    apply (rule beval_world_raw_cases[OF *])
+    apply (erule beval_cases)+
+    using \<open>3 < len\<close> **  by simp
+qed
+
+lemma index_seq_hoare_next_time:
+  assumes "seq_wt \<Gamma> (Bassign_trans OUT (Bindex IN 3) 1)"
+  shows   "\<turnstile> [\<lambda>tw. inv tw \<and> wityping \<Gamma> (snd tw)] Bassign_trans OUT (Bindex IN 3) 1 [\<lambda>tw. inv (next_time_world tw, snd tw)]"
+  apply (rule Assign2_altI)
+  using inv_next_time type_correctness_length[OF assms] by blast
+
+lemma index_seq_hoare_next_time0:
+  assumes "seq_wt \<Gamma> (Bassign_trans OUT (Bindex IN 3) 1)"
+  shows   "\<turnstile> [\<lambda>tw. fst tw = 0 \<and> wityping \<Gamma> (snd tw)] Bassign_trans OUT (Bindex IN 3) 1 [\<lambda>tw. inv (next_time_world tw, snd tw)]"
+  apply (rule Assign2_altI)
+  using inv_next_time type_correctness_length[OF assms]  Indexing_Hoare.inv_def gr_implies_not_zero
+  by blast
+
+lemma index_conc_hoare:
+  "\<And>tw. inv tw \<and> inv' tw \<and> disjnt {IN} (event_of tw) \<Longrightarrow> inv (next_time_world tw, snd tw)"
+  by (smt inv_def comp_apply inv'_def not_less prod.sel(1) snd_conv
+  unchanged_until_next_time_world)
+
+lemma index_conc_hoare2:
+  "\<And>tw. inv tw \<and> inv' tw \<and> disjnt {IN} (event_of tw) \<Longrightarrow> inv' (next_time_world tw, snd tw)"
+  unfolding inv_def inv'_def
+  by (smt Suc_diff_1 comp_apply diff_less disjnt_insert1 event_of_alt_def gr_implies_not_zero
+  le_Suc_eq le_less_trans mem_Collect_eq next_time_world_at_least not_less order.strict_iff_order
+  prod.sel(1) snd_conv unchanged_until_next_time_world zero_less_one)
+
+lemma inv'_next_time:
+  fixes tw
+  assumes "beval_world_raw2 tw (Bindex IN 3) x" and "type_of x = Bty"
+  defines "tw' \<equiv> tw[OUT, 1 :=\<^sub>2 x]"
+  shows   "inv' (next_time_world tw', snd tw')"
+  unfolding inv'_def
+proof (rule, rule, rule)
+  fix i
+  assume "disjnt {IN} (event_of (next_time_world tw', snd tw'))"
+  hence "IN \<notin> event_of (next_time_world tw', snd tw')"
+    by auto
+  assume "fst (next_time_world tw', snd tw') \<le> i"
+  hence "next_time_world tw' \<le> i"
+    by auto
+  let ?t' = "next_time_world tw'"
+  have "fst tw' < ?t'"
+    using next_time_world_at_least by blast
+  moreover have "fst tw = fst tw'"
+    unfolding tw'_def unfolding worldline_upd2_def by auto
+  ultimately have "fst tw < ?t'"
+    by auto
+  have "wline_of (?t', snd tw') OUT (i + 1) = wline_of tw' OUT (i + 1)"
+    by auto
+  also have "... = x"
+    unfolding tw'_def worldline_upd2_def worldline_upd_def using \<open>next_time_world tw' \<le> i\<close> \<open>fst tw < ?t'\<close>
+    by auto
+  also have "bval_of ... = lof_wline tw IN (fst tw) ! 3"
+  proof -
+    have assm: "beval_world_raw (snd tw) (fst tw) (Bindex IN 3) x"
+      using assms(1) unfolding beval_world_raw2_def by auto
+    show ?thesis
+      apply (rule beval_world_raw_cases[OF assm])
+      apply (erule beval_cases)+
+      by (metis comp_apply state_of_world_def val.sel(1) val.sel(2))
+  qed
+  also have "... = lof_wline tw IN (fst tw') ! 3"
+    unfolding tw'_def worldline_upd2_def worldline_upd_def by auto
+  also have "... = lof_wline tw' IN (?t') ! 3"
+  proof -
+    have "wline_of tw' IN ?t' = wline_of tw' IN (?t' - 1)"
+      using \<open>IN \<notin> event_of (?t', snd tw')\<close> unfolding event_of_alt_def
+      using \<open>get_time tw < next_time_world tw'\<close> by auto
+    also have "... = wline_of tw' IN (fst tw')"
+      using unchanged_until_next_time_world
+      by (metis (no_types, lifting) Suc_diff_1 \<open>get_time tw' < next_time_world tw'\<close> diff_less
+      gr_implies_not_zero le_0_eq less_Suc_eq_le not_less zero_less_one)
+    also have "... = wline_of tw' IN (fst tw)"
+      by (simp add: \<open>get_time tw = get_time tw'\<close>)
+    also have "... = wline_of tw IN (fst tw)"
+      unfolding tw'_def worldline_upd2_def worldline_upd_def by simp
+    finally have "wline_of tw' IN ?t' = wline_of tw IN (fst tw)"
+      by auto
+    thus ?thesis
+      using \<open>fst tw = fst tw'\<close> by simp
+  qed
+  also have "... = lof_wline (?t', snd tw') IN ?t' ! 3"
+    by auto
+  finally show "bof_wline (next_time_world tw', snd tw') OUT (i + 1) = lof_wline (next_time_world tw', snd tw') IN (get_time (next_time_world tw', snd tw')) ! 3"
+    by simp
+qed
+
+lemma index_seq_hoare_next_time1:
+  assumes "seq_wt \<Gamma> (Bassign_trans OUT (Bindex IN 3) 1)"
+  shows   "\<turnstile> [\<lambda>tw. wityping \<Gamma> (snd tw)] Bassign_trans OUT (Bindex IN 3) 1 [\<lambda>tw. inv' (next_time_world tw, snd tw)]"
+  apply (rule Assign2_altI)
+  using inv'_next_time type_correctness_length[OF assms] by blast
+
+lemma index_conc_hoare3:
+  assumes "seq_wt \<Gamma> (Bassign_trans OUT (Bindex IN 3) 1)"
+  shows "\<turnstile> \<lbrace>\<lambda>tw. (inv tw \<and> wityping \<Gamma> (snd tw)) \<and> inv' tw\<rbrace> index \<lbrace>\<lambda>tw. inv (next_time_world tw, snd tw) \<and> inv' (next_time_world tw, snd tw)\<rbrace>"
+  unfolding index_def
+  apply (rule Single)
+   apply (rule Conj)
+    apply (rule strengthen_precondition)
+    apply (rule strengthen_precondition)
+    apply(rule index_seq_hoare_next_time[OF assms])
+   apply (rule strengthen_precondition)
+   apply (rule strengthen_precondition)
+   apply (rule strengthen_precondition2)
+   apply(rule index_seq_hoare_next_time1[OF assms])
+  using index_conc_hoare index_conc_hoare2 by blast
+
+lemma index_conc_hoare4:
+  assumes "seq_wt \<Gamma> (Bassign_trans OUT (Bindex IN 3) 1)"
+  shows "\<turnstile> \<lbrace>\<lambda>tw. (inv tw \<and> wityping \<Gamma> (snd tw)) \<and> inv' tw\<rbrace> index \<lbrace>\<lambda>tw. (inv (next_time_world tw, snd tw) \<and> wityping \<Gamma> (snd tw)) \<and> inv' (next_time_world tw, snd tw)\<rbrace>"
+  apply (rule Conj2)
+   apply (rule Conj2)
+    apply (rule weaken_post_conc_hoare[OF _ index_conc_hoare3[OF assms]])
+    apply blast
+   apply (rule strengthen_pre_conc_hoare[rotated])
+    apply (unfold index_def, rule single_conc_stmt_preserve_wityping_hoare[OF assms], blast)
+  apply (fold index_def, rule weaken_post_conc_hoare[OF _ index_conc_hoare3[OF assms]], blast)
+  done
+
+lemma index_conc_sim':
+  assumes "seq_wt \<Gamma> (Bassign_trans OUT (Bindex IN 3) 1)"
+  shows   "\<turnstile>\<^sub>s \<lbrace>\<lambda>tw. (inv tw \<and> wityping \<Gamma> (snd tw)) \<and> inv' tw\<rbrace> index \<lbrace>\<lambda>tw. (inv tw \<and> wityping \<Gamma> (snd tw)) \<and> inv' tw\<rbrace>"
+  apply (rule While)
+  apply (unfold snd_conv, rule index_conc_hoare4[OF assms])
+  done
+
+lemma index_conc_sim2':
+  assumes "seq_wt \<Gamma> (Bassign_trans OUT (Bindex IN 3) 1)"
+  shows   "\<turnstile>\<^sub>s \<lbrace>\<lambda>tw. (inv tw \<and> wityping \<Gamma> (snd tw)) \<and> inv' tw\<rbrace> index \<lbrace>inv\<rbrace>"
+  using index_conc_sim' Conseq_sim assms by smt
+
+lemma init_sat_index_inv:
+  assumes "seq_wt \<Gamma> (Bassign_trans OUT (Bindex IN 3) 1)"
+  shows   "init_sim_hoare (\<lambda>tw. fst tw = 0 \<and> wityping \<Gamma> (snd tw)) index (\<lambda>tw. inv tw \<and> wityping \<Gamma> (snd tw))"
+  unfolding index_def
+  apply (rule AssignI)
+  apply (rule SingleI)
+  apply (rule Conj)
+  unfolding snd_conv apply (rule index_seq_hoare_next_time0[OF assms])
+  apply (rule strengthen_precondition2)
+  by (metis assms seq_stmt_preserve_wityping_hoare)
+
+lemma init_sat_index_inv2:
+  assumes "seq_wt \<Gamma> (Bassign_trans OUT (Bindex IN 3) 1)"
+  shows "init_sim_hoare (\<lambda>tw. wityping \<Gamma> (snd tw)) index inv'"
+  unfolding index_def
+  apply (rule AssignI)
+  apply (rule SingleI)
+  unfolding snd_conv apply (rule index_seq_hoare_next_time1[OF assms])
+  done
+
+lemma init_sat_slicer_inv_comb:
+  assumes "seq_wt \<Gamma> (Bassign_trans OUT (Bindex IN 3) 1)"
+  shows   "init_sim_hoare (\<lambda>tw. fst tw = 0 \<and> wityping \<Gamma> (snd tw)) index (\<lambda>tw. (inv tw \<and> wityping \<Gamma> (snd tw)) \<and> inv' tw)"
+  apply (rule ConjI_sim)
+  apply (rule init_sat_index_inv[OF assms])
+  apply (rule ConseqI_sim[rotated])
+  apply (rule init_sat_index_inv2[OF assms])
+  by blast+
+
+lemma slicer_correctness:
+  assumes "sim_fin w (i + 1) index tw'" and "wityping \<Gamma> w"
+  assumes "conc_wt \<Gamma> index"
+  shows   "bof_wline tw' OUT (i + 1) = lof_wline tw' IN i ! 3"
+proof -
+  obtain tw where "init_sim (0, w) index tw" and  "tw, i + 1, index \<Rightarrow>\<^sub>S tw'"
+    using premises_sim_fin_obt[OF assms(1)] by auto
+  hence "i + 1 < fst tw'"
+    using world_maxtime_lt_fst_tres  by blast
+  have "conc_stmt_wf index"
+    unfolding conc_stmt_wf_def index_def by auto
+  moreover have "nonneg_delay_conc index"
+    unfolding index_def by auto
+  ultimately have "init_sim_valid (\<lambda>tw. fst tw = 0 \<and> wityping \<Gamma> (snd tw)) index (\<lambda>tw. (inv tw \<and> wityping \<Gamma> (snd tw)) \<and> inv' tw)"
+    using init_sim_hoare_soundness[OF init_sat_slicer_inv_comb]
+    by (metis (no_types, lifting) assms(3) conc_wt_cases(1) init_sat_slicer_inv_comb
+    init_sim_hoare_soundness index_def strengthen_precondition_init_sim_hoare)
+  hence "inv tw \<and> wityping \<Gamma> (snd tw) \<and> inv' tw"
+    using \<open>init_sim (0, w) index tw\<close> fst_conv assms(2) unfolding init_sim_valid_def
+    by (metis snd_conv)
+  hence "inv tw" and "inv' tw" and "wityping \<Gamma> (snd tw)"
+    by auto
+  moreover have "seq_wt \<Gamma> (Bassign_trans OUT (Bindex IN 3) 1)"
+    using assms(3) unfolding index_def by auto
+  moreover hence "\<Turnstile>\<^sub>s \<lbrace>\<lambda>tw. (inv tw \<and> wityping \<Gamma> (snd tw)) \<and> inv' tw\<rbrace> index \<lbrace>inv\<rbrace>"
+    using conc_sim_soundness[OF index_conc_sim2'] \<open>conc_stmt_wf index\<close> \<open>nonneg_delay_conc index\<close>
+    by auto
+  ultimately have "inv tw'"
+    using \<open>tw, i + 1, index \<Rightarrow>\<^sub>S tw'\<close> unfolding sim_hoare_valid_def by blast
+  with \<open>i + 1 < fst tw'\<close> show ?thesis
+    unfolding inv_def by auto
+qed
+
+end
