Slicing_Hoare.thy
@@ -1,0 +1,417 @@
+(*
+ * Copyright 2019, NTU
+ *
+ * This software may be distributed and modified according to the terms of
+ * the BSD 2-Clause license. Note that NO WARRANTY is provided.
+ * See "LICENSE_BSD2.txt" for details.
+ *
+ *  Author: Albert Rizaldi, NTU Singapore
+ *)
+
+theory Slicing_Hoare
+  imports VHDL_Hoare_Complete
+begin
+
+datatype sig = IN | OUT
+
+definition slicer :: "sig conc_stmt" where
+  "slicer = process {IN} : Bassign_trans OUT (Bslice IN 3 2) 1"
+
+lemma potential_tyenv:
+  assumes "seq_wt \<Gamma> (Bassign_trans OUT (Bslice IN 3 2) 1)"
+  shows "\<exists>len>3. \<Gamma> IN = Lty len \<and> \<Gamma> OUT = Lty 2"
+proof (rule seq_wt_cases(4)[OF assms])
+  assume "bexp_wt \<Gamma> (Bslice IN 3 2) (\<Gamma> OUT)"
+  then obtain len where "bexp_wt \<Gamma> (Bsig IN) (Lty len) \<and> 3 < len \<and> \<Gamma> OUT = Lty 2"
+    by (metis add_2_eq_Suc add_Suc add_Suc_right add_diff_cancel_right' bexp_wt_cases(8)
+    numeral_2_eq_2 numeral_3_eq_3)
+  hence "bexp_wt \<Gamma> (Bsig IN) (Lty len)" and "3 < len" and "\<Gamma> OUT = Lty 2"
+    by auto
+  hence "\<Gamma> IN = Lty len"
+    using bexp_wt_cases(9)[OF \<open>bexp_wt \<Gamma> (Bsig IN) (Lty len)\<close>] by metis
+  thus ?thesis
+    using \<open>3 < len\<close> \<open>\<Gamma> OUT = Lty 2\<close> by blast
+qed
+
+abbreviation "lof_wline tw sig i \<equiv> lval_of (wline_of tw sig i)"
+
+definition inv :: "sig assn2" where
+  "inv tw = (\<forall>i < fst tw. let ins = lof_wline tw IN i; idx = length ins - 1 in 
+                                          lof_wline tw OUT (i + 1) = nths ins {idx - 3 .. idx - 2})"
+
+definition inv' :: "sig assn2" where
+  "inv' tw = (disjnt {IN} (event_of tw) \<longrightarrow> 
+              (\<forall>i\<ge>fst tw. let ins = lof_wline tw IN (fst tw); idx = length ins - 1 in 
+                                         lof_wline tw OUT (i + 1) = nths ins {idx - 3 .. idx - 2}))"
+
+text \<open>Note that we need the assumption that @{term "type_of x = Lty 2"} as there is no
+guarantee that @{term "beval_world_raw2 tw (Bslice IN 3 2) x"} would result in a list 
+of length 2.\<close>
+
+lemma inv_next_time:
+  assumes "inv tw"
+  assumes "beval_world_raw2 tw (Bslice IN 3 2) x" and "type_of x = Lty 2"
+  defines "tw' \<equiv> tw[OUT, 1 :=\<^sub>2 x]"
+  shows   "inv (next_time_world tw', snd tw')"
+proof -
+  have "fst tw' < next_time_world tw'"
+    using next_time_world_at_least  using nat_less_le by blast
+  moreover have "fst tw = fst tw'"
+    unfolding tw'_def worldline_upd2_def worldline_upd_def by auto
+  ultimately have "fst tw < next_time_world tw'"
+    by auto
+  have "\<forall>i < next_time_world tw'. let ins = lof_wline tw' IN i; idx = length ins - 1 in
+                                           lof_wline tw' OUT (i + 1) = nths ins {idx - 3 .. idx - 2}"
+  proof (rule, rule)
+    fix i 
+    let ?ins   = "lof_wline tw IN i"
+    let ?ins'  = "lof_wline tw' IN i"
+    let ?instw = "lof_wline tw IN (fst tw)"
+    let ?idx   = "length ?ins - 1"
+    let ?idx'  = "length ?ins' - 1"
+    let ?idxtw = "length ?instw - 1"
+
+    assume "i < next_time_world tw'"
+    hence "i < fst tw \<or> fst tw \<le> i \<and> i < next_time_world tw' - 1 \<or> i = next_time_world tw' - 1"
+      using \<open>fst tw < next_time_world tw'\<close> by auto
+    moreover
+    { assume "i < fst tw"
+      have "lof_wline tw' OUT (i + 1) = lof_wline tw OUT (i + 1)"
+        using \<open>i < fst tw\<close> \<open>fst tw < next_time_world tw'\<close> unfolding tw'_def worldline_upd2_def
+        worldline_upd_def by (simp add: discrete)
+      also have "... = nths ?ins {?idx - 3 .. ?idx - 2}"
+        using assms(1) \<open>i < fst tw\<close> unfolding inv_def Let_def by auto
+      also have "... = nths ?ins' {?idx' - 3 .. ?idx' - 2}"
+      proof -
+        have "lof_wline tw' IN i = lof_wline tw IN i"
+          using \<open>i < fst tw\<close> \<open>fst tw < next_time_world tw'\<close> unfolding tw'_def worldline_upd2_def
+          worldline_upd_def by (simp add: discrete)
+        thus ?thesis
+          by auto
+      qed
+      finally have "lof_wline tw' OUT (i + 1) = nths ?ins' {?idx' - 3 .. ?idx' - 2}"
+        by auto }
+    moreover
+    { assume "fst tw \<le> i \<and> i < next_time_world tw' - 1"
+      hence "lof_wline tw' OUT (i + 1) = lof_wline tw' OUT (fst tw + 1)"
+        using unchanged_until_next_time_world
+        by (metis (mono_tags, lifting) Suc_eq_plus1 \<open>get_time tw = get_time tw'\<close> le_Suc_eq le_add1
+        le_less_trans less_diff_conv)      
+      have "lof_wline tw' IN i = lof_wline tw IN (fst tw)"
+        using unchanged_until_next_time_world 
+        by (metis \<open>get_time tw = get_time tw'\<close> \<open>get_time tw \<le> i \<and> i < next_time_world tw' - 1\<close> \<open>i <
+        next_time_world tw'\<close> less_add_one tw'_def worldline_upd2_before_dly)
+      let ?instw = "lof_wline tw IN (fst tw)"
+      let ?idxtw = "length ?instw - 1"
+      have "nths ?ins' {?idx' - 3 .. ?idx' - 2} = nths ?instw {?idxtw - 3 .. ?idxtw - 2}"
+        using \<open>lof_wline tw' IN i = lof_wline tw IN (fst tw)\<close> by simp
+      have "lof_wline tw' OUT (fst tw + 1) = lval_of x"  
+        using assms(4)  by (metis worldline_upd2_at_dly)
+      also have "... = nths ?instw {?idxtw - 3 .. ?idxtw - 2}"
+      proof -
+        have assms2: "beval_world_raw (snd tw) (fst tw) (Bslice IN 3 2) x"
+          using assms(2) unfolding beval_world_raw2_def by auto
+        have "\<not> is_Bv (wline_of tw IN (fst tw))"
+          apply (rule beval_world_raw_cases[OF assms2], erule beval_cases)
+          by (metis beval_cases(1) comp_apply state_of_world_def val.disc(2))
+        hence "state_of_world (snd tw) (fst tw) IN = Lv ?instw"
+          unfolding state_of_world_def by simp
+        show "lval_of x = nths ?instw {?idxtw - 3 .. ?idxtw - 2}"
+          apply (rule beval_world_raw_cases[OF assms2], erule beval_cases)
+          using \<open>state_of_world (snd tw) (fst tw) IN = Lv ?instw\<close> plus_1_eq_Suc by auto
+      qed
+      also have "... = nths ?ins' {?idx' - 3 .. ?idx' - 2}"
+        using \<open>lof_wline tw' IN i = lof_wline tw IN (fst tw)\<close>
+        by simp
+      finally have "lof_wline tw' OUT (i + 1) = nths ?ins' {?idx' - 3 .. ?idx' - 2}"
+        using \<open>lof_wline tw' OUT (i + 1) = lof_wline tw' OUT (fst tw + 1)\<close> by auto }
+    moreover
+    { assume "i = next_time_world tw' - 1"
+      hence "lof_wline tw' OUT (i + 1) = lof_wline tw' OUT (next_time_world tw')"
+        using \<open>i < next_time_world tw'\<close> by auto
+      also have "... = lof_wline tw' OUT (fst tw' + 1)"
+        by (smt Suc_eq_plus1 \<open>get_time tw < next_time_world tw'\<close> \<open>get_time tw = get_time tw'\<close>
+        comp_def dual_order.strict_trans1 less_Suc_eq_le less_not_refl snd_conv tw'_def
+        worldline_upd2_def worldline_upd_def)
+      also have "... = lof_wline tw' OUT (fst tw + 1)"
+        unfolding `fst tw = fst tw'` by auto
+      also have "... = lval_of x"
+        using assms(4)  by (metis worldline_upd2_at_dly)
+      also have "... = nths ?instw {?idxtw - 3 .. ?idxtw - 2}"
+      proof -
+        have assms2: "beval_world_raw (snd tw) (fst tw) (Bslice IN 3 2) x"
+          using assms(2) unfolding beval_world_raw2_def by auto
+        have "\<not> is_Bv (wline_of tw IN (fst tw))"
+          apply (rule beval_world_raw_cases[OF assms2], erule beval_cases)
+          by (metis beval_cases(1) comp_apply state_of_world_def val.disc(2))
+        hence "state_of_world (snd tw) (fst tw) IN = Lv ?instw"
+          unfolding state_of_world_def by simp
+        show "lval_of x = nths ?instw {?idxtw - 3 .. ?idxtw - 2}"
+          apply (rule beval_world_raw_cases[OF assms2], erule beval_cases)
+          using \<open>state_of_world (snd tw) (fst tw) IN = Lv ?instw\<close> plus_1_eq_Suc by auto
+      qed
+      also have "... = nths ?ins' {?idx' - 3 .. ?idx' - 2}"
+        by (smt \<open>get_time tw = get_time tw'\<close> \<open>i < get_time tw \<Longrightarrow> lof_wline tw' OUT (i + 1) = nths
+        (lof_wline tw' IN i) {length (lof_wline tw' IN i) - 1 - 3..length (lof_wline tw' IN i) - 1 -
+        2}\<close> \<open>i < next_time_world tw'\<close> calculation comp_def not_less sig.distinct(1) snd_conv tw'_def
+        unchanged_until_next_time_world worldline_upd2_def worldline_upd_def)
+      finally have "lof_wline tw' OUT (i + 1) = nths ?ins' {?idx' - 3 .. ?idx' - 2}"
+        by blast }
+    ultimately show "let ins = lof_wline tw' IN i; idx = length ins - 1 in lof_wline tw' OUT (i + 1) = nths ins {idx - 3..idx - 2}"
+      unfolding Let_def by auto
+  qed
+  thus ?thesis
+    unfolding inv_def by auto
+qed
+
+lemma type_correctness_length:
+  assumes "seq_wt \<Gamma> (Bassign_trans OUT (Bslice IN 3 2) 1)"
+  assumes "wityping \<Gamma> (snd tw)"
+  assumes "beval_world_raw2 tw (Bslice IN 3 2) x"
+  shows   "type_of x = Lty 2"
+proof - 
+  obtain len where "\<Gamma> IN = Lty len" and "3 < len"
+    using potential_tyenv[OF assms(1)] by auto
+  have *: "beval_world_raw (snd tw) (fst tw) (Bslice IN 3 2) x"
+    using assms(3) unfolding beval_world_raw2_def by auto
+  have "type_of (state_of_world (snd tw) (get_time tw) IN) = Lty len"
+    using assms(2) unfolding wityping_def 
+    by (simp add: \<open>\<Gamma> IN = Lty len\<close> state_of_world_def wtyping_def)
+  hence **: "\<And>bs. state_of_world (snd tw) (fst tw) IN = Lv bs \<Longrightarrow> length bs = len"
+    by simp
+  have ***: "\<And>bs. 3 < length bs  \<Longrightarrow> length (nths bs {length bs - Suc 3..length bs - Suc 2}) = 2"
+  proof -
+    fix bs :: "'a list"
+    assume "3 < length bs"
+    hence "length (nths bs {length bs - Suc 3..length bs - Suc 2}) = 
+                               card {i. i < length bs \<and> i \<in> {length bs - Suc 3..length bs - Suc 2}}"
+      unfolding length_nths by auto
+    have "\<And>i. i \<in> {length bs - Suc 3 .. length bs - Suc 2} \<Longrightarrow> i < length bs"
+      using \<open>3 < length bs\<close> by auto
+    hence "{i. i < length bs \<and> i \<in> {length bs - Suc 3 .. length bs - Suc 2}} = 
+           {i. i \<in> {length bs - Suc 3 .. length bs - Suc 2}}" (is "?lhs = ?rhs")
+      by auto
+    hence "card ?lhs = card ?rhs"
+      by auto
+    also have "... = 2"
+      using \<open>3 < length bs\<close> 
+      by (metis Collect_mem_eq One_nat_def Suc_diff_Suc Suc_numeral add_diff_cancel_left'
+      add_diff_cancel_right' card_atLeastAtMost diff_less_Suc numeral_2_eq_2 plus_1_eq_Suc
+      semiring_norm(5))
+    finally have "card ?lhs = 2"
+      by auto
+    thus "length (nths bs {length bs - Suc 3..length bs - Suc 2}) = 2 "
+      using \<open>length (nths bs {length bs - Suc 3..length bs - Suc 2}) = card {i. i < length bs \<and> i \<in>
+      {length bs - Suc 3..length bs - Suc 2}}\<close> by linarith
+  qed
+  show ?thesis
+    apply (rule beval_world_raw_cases[OF *])
+    apply (erule beval_cases)+
+    using \<open>3 < len\<close> ** ***  by force
+qed
+
+lemma slicer_seq_hoare_next_time:
+  assumes "seq_wt \<Gamma> (Bassign_trans OUT (Bslice IN 3 2) 1)"
+  shows "\<turnstile> [\<lambda>tw. inv tw \<and> wityping \<Gamma> (snd tw)]  Bassign_trans OUT (Bslice IN 3 2) 1 [\<lambda>tw. inv (next_time_world tw, snd tw)]"
+  apply (rule Assign2_altI)
+  using inv_next_time type_correctness_length[OF assms] by blast
+
+lemma slicer_seq_hoare_next_time0:
+  assumes "seq_wt \<Gamma> (Bassign_trans OUT (Bslice IN 3 2) 1)"
+  shows "\<turnstile> [\<lambda>tw. fst tw = 0 \<and> wityping \<Gamma> (snd tw)] Bassign_trans OUT (Bslice IN 3 2) 1 [\<lambda>tw. inv (next_time_world tw, snd tw)]"
+  apply (rule Assign2_altI)
+  using inv_next_time type_correctness_length[OF assms] inv_def gr_implies_not0 by blast
+
+lemma slicer_conc_hoare:
+  "\<And>tw. inv tw \<and> inv' tw \<and> disjnt {IN} (event_of tw) \<Longrightarrow> inv (next_time_world tw, snd tw)"
+  by (smt Slicing_Hoare.inv_def comp_apply inv'_def not_less prod.sel(1) snd_conv
+  unchanged_until_next_time_world)
+
+lemma slicer_conc_hoare2:
+  "\<And>tw. inv tw \<and> inv' tw \<and> disjnt {IN} (event_of tw) \<Longrightarrow> inv' (next_time_world tw, snd tw)"
+  unfolding inv_def inv'_def 
+  by (smt Suc_diff_1 comp_apply diff_less disjnt_insert1 event_of_alt_def gr_implies_not_zero
+  le_Suc_eq le_less_trans mem_Collect_eq next_time_world_at_least not_less order.strict_iff_order
+  prod.sel(1) snd_conv unchanged_until_next_time_world zero_less_one)
+
+lemma inv'_next_time:
+  fixes tw
+  assumes "beval_world_raw2 tw (Bslice IN 3 2) x" and "type_of x = Lty 2"
+  defines "tw' \<equiv> tw[OUT, 1 :=\<^sub>2 x]"
+  shows   "inv' (next_time_world tw', snd tw')"
+  unfolding inv'_def
+proof (rule, rule, rule)
+  fix i
+  assume "disjnt {IN} (event_of (next_time_world tw', snd tw'))"
+  hence "IN \<notin> event_of (next_time_world tw', snd tw')"
+    by auto
+  assume "fst (next_time_world tw', snd tw') \<le> i"
+  hence "next_time_world tw' \<le> i"
+    by auto
+  let ?ins = "lof_wline (next_time_world tw', snd tw') IN (next_time_world tw')"
+  let ?idx = "length ?ins - 1"
+
+  let ?t' = "next_time_world tw'"
+  have "fst tw' < ?t'"
+    using next_time_world_at_least by blast
+  moreover have "fst tw = fst tw'"
+    unfolding tw'_def unfolding worldline_upd2_def by auto
+  ultimately have "fst tw < ?t'"
+    by auto
+  have "wline_of tw' IN ?t' = wline_of tw IN (fst tw)"
+  proof -
+    have "wline_of tw' IN ?t' = wline_of tw' IN (?t' - 1)"
+      using \<open>IN \<notin> event_of (?t', snd tw')\<close> unfolding event_of_alt_def
+      using \<open>get_time tw < next_time_world tw'\<close> by auto
+    also have "... = wline_of tw' IN (fst tw')"
+      using unchanged_until_next_time_world 
+      by (metis (no_types, lifting) Suc_diff_1 \<open>get_time tw' < next_time_world tw'\<close> diff_less
+      gr_implies_not_zero le_0_eq less_Suc_eq_le not_less zero_less_one)
+    also have "... = wline_of tw' IN (fst tw)"
+      by (simp add: \<open>get_time tw = get_time tw'\<close>)
+    also have "... = wline_of tw IN (fst tw)"
+      unfolding tw'_def worldline_upd2_def worldline_upd_def by simp
+    finally show "wline_of tw' IN ?t' = wline_of tw IN (fst tw)"
+      by auto
+  qed
+  moreover have "?ins = lof_wline tw' IN ?t'"
+    by auto
+  ultimately have "?ins = lof_wline tw IN (fst tw)"
+    by auto
+  have "\<And>i. ?t' \<le> i \<Longrightarrow> lof_wline tw' OUT (i + 1) = nths ?ins {?idx - 3 .. ?idx - 2}"
+  proof -
+    fix i
+    have assms2: "beval_world_raw (snd tw) (fst tw) (Bslice IN 3 2) x"
+      using assms unfolding beval_world_raw2_def by auto
+    assume "?t' \<le> i"
+    hence "lof_wline tw' OUT (i + 1) = lval_of x"
+      using `fst tw < ?t'`
+      unfolding tw'_def worldline_upd2_def worldline_upd_def by auto
+    have "\<not> is_Bv (wline_of tw IN (fst tw))"
+      by (rule beval_world_raw_cases[OF assms2], erule beval_cases)
+         (metis beval_cases(1) comp_apply state_of_world_def val.disc(2))
+    hence "state_of_world (snd tw) (fst tw) IN = Lv ?ins"
+      unfolding \<open>?ins = lof_wline tw IN (fst tw)\<close>state_of_world_def by simp
+    have "lval_of x = nths ?ins {?idx - 3 .. ?idx - 2}"
+      apply (rule beval_world_raw_cases[OF assms2])  
+      apply (erule beval_cases)+
+      using \<open>state_of_world (snd tw) (fst tw) IN = Lv ?ins\<close> 
+      by (metis \<open>lof_wline (next_time_world tw', snd tw') IN (next_time_world tw') = lof_wline tw IN
+      (get_time tw)\<close> diff_Suc_eq_diff_pred eval_nat_numeral(3) val.sel(2))
+    thus "lof_wline tw' OUT (i + 1) = nths ?ins {?idx - 3 .. ?idx - 2}"
+      using \<open>lof_wline tw' OUT (i + 1) = lval_of x\<close> by auto
+  qed
+  thus "let ins = lof_wline (next_time_world tw', snd tw') IN (get_time (next_time_world tw', snd tw')); idx = length ins - 1
+         in lof_wline (next_time_world tw', snd tw') OUT (i + 1) = nths ins {idx - 3..idx - 2}"
+    by (simp add: \<open>next_time_world tw' \<le> i\<close>)
+qed
+
+lemma slicer_seq_hoare_next_time1:
+  assumes "seq_wt \<Gamma> (Bassign_trans OUT (Bslice IN 3 2) 1)"
+  shows "\<turnstile> [\<lambda>tw. wityping \<Gamma> (snd tw)] Bassign_trans OUT (Bslice IN 3 2) 1 [\<lambda>tw. inv' (next_time_world tw, snd tw)]"
+  apply (rule Assign2_altI)
+  using inv'_next_time type_correctness_length[OF assms] by blast
+
+lemma slicer_conc_hoare3:
+  assumes "seq_wt \<Gamma> (Bassign_trans OUT (Bslice IN 3 2) 1)"
+  shows "\<turnstile> \<lbrace>\<lambda>tw. (inv tw \<and> wityping \<Gamma> (snd tw)) \<and> inv' tw\<rbrace> slicer \<lbrace>\<lambda>tw. inv (next_time_world tw, snd tw) \<and> inv' (next_time_world tw, snd tw)\<rbrace>"
+  unfolding slicer_def
+  apply (rule Single)
+   apply (rule Conj)
+  apply (rule strengthen_precondition)    
+    apply (rule strengthen_precondition)
+    apply (rule slicer_seq_hoare_next_time[OF assms])
+   apply (rule strengthen_precondition)
+   apply (rule strengthen_precondition)
+   apply (rule strengthen_precondition2)
+   apply (rule slicer_seq_hoare_next_time1[OF assms])
+  using slicer_conc_hoare slicer_conc_hoare2 by blast
+
+lemma slicer_conc_hoare4:
+  assumes "seq_wt \<Gamma> (Bassign_trans OUT (Bslice IN 3 2) 1)"
+  shows "\<turnstile> \<lbrace>\<lambda>tw. (inv tw \<and> wityping \<Gamma> (snd tw)) \<and> inv' tw\<rbrace> slicer \<lbrace>\<lambda>tw. (inv (next_time_world tw, snd tw) \<and> wityping \<Gamma> (snd tw)) \<and> inv' (next_time_world tw, snd tw)\<rbrace>"
+  apply (rule Conj2)
+   apply (rule Conj2)
+    apply (rule weaken_post_conc_hoare[OF _ slicer_conc_hoare3[OF assms]])
+    apply blast
+   apply (rule strengthen_pre_conc_hoare[rotated])
+    apply (unfold slicer_def, rule single_conc_stmt_preserve_wityping_hoare[OF assms], blast)
+  apply (fold slicer_def, rule weaken_post_conc_hoare[OF _ slicer_conc_hoare3[OF assms]], blast)
+  done
+  
+lemma slicer_conc_sim':
+  assumes "seq_wt \<Gamma> (Bassign_trans OUT (Bslice IN 3 2) 1)"
+  shows   "\<turnstile>\<^sub>s \<lbrace>\<lambda>tw. (inv tw \<and> wityping \<Gamma> (snd tw)) \<and> inv' tw\<rbrace> slicer \<lbrace>\<lambda>tw. (inv tw \<and> wityping \<Gamma> (snd tw)) \<and> inv' tw\<rbrace>"
+  apply (rule While)
+  apply (unfold snd_conv, rule slicer_conc_hoare4[OF assms])
+  done
+
+lemma slicer_conc_sim2':
+  assumes "seq_wt \<Gamma> (Bassign_trans OUT (Bslice IN 3 2) 1)"
+  shows   "\<turnstile>\<^sub>s \<lbrace>\<lambda>tw. (inv tw \<and> wityping \<Gamma> (snd tw)) \<and> inv' tw\<rbrace> slicer \<lbrace>inv\<rbrace>"
+  using slicer_conc_sim' Conseq_sim assms by smt
+
+lemma init_sat_slicer_inv:
+  assumes "seq_wt \<Gamma> (Bassign_trans OUT (Bslice IN 3 2) 1)"
+  shows   "init_sim_hoare (\<lambda>tw. fst tw = 0 \<and> wityping \<Gamma> (snd tw)) slicer (\<lambda>tw. inv tw \<and> wityping \<Gamma> (snd tw))"
+  unfolding slicer_def
+  apply (rule AssignI)
+  apply (rule SingleI)
+  apply (rule Conj)
+  unfolding snd_conv apply (rule slicer_seq_hoare_next_time0[OF assms])
+  apply (rule strengthen_precondition2)
+  by (metis assms seq_stmt_preserve_wityping_hoare)
+
+lemma init_sat_slicer_inv2:
+  assumes "seq_wt \<Gamma> (Bassign_trans OUT (Bslice IN 3 2) 1)"
+  shows "init_sim_hoare (\<lambda>tw. wityping \<Gamma> (snd tw)) slicer inv'"
+  unfolding slicer_def
+  apply (rule AssignI)
+  apply (rule SingleI)
+  unfolding snd_conv apply (rule slicer_seq_hoare_next_time1[OF assms])
+  done
+
+lemma init_sat_slicer_inv_comb:
+  assumes "seq_wt \<Gamma> (Bassign_trans OUT (Bslice IN 3 2) 1)"
+  shows   "init_sim_hoare (\<lambda>tw. fst tw = 0 \<and> wityping \<Gamma> (snd tw)) slicer (\<lambda>tw. (inv tw \<and> wityping \<Gamma> (snd tw)) \<and> inv' tw)"
+  apply (rule ConjI_sim)
+  apply (rule init_sat_slicer_inv[OF assms])
+  apply (rule ConseqI_sim[rotated])
+  apply (rule init_sat_slicer_inv2[OF assms])
+  by blast+
+
+lemma slicer_correctness:
+  assumes "sim_fin w (i + 1) slicer tw'" and "wityping \<Gamma> w"
+  assumes "conc_wt \<Gamma> slicer"
+  shows   "let ins = lof_wline tw' IN i; idx = length ins - 1 in 
+                                          lof_wline tw' OUT (i + 1) = nths ins {idx - 3 .. idx - 2}"
+proof -
+  obtain tw where "init_sim (0, w) slicer tw" and  "tw, i + 1, slicer \<Rightarrow>\<^sub>S tw'"
+    using premises_sim_fin_obt[OF assms(1)] by auto
+  hence "i + 1 < fst tw'"
+    using world_maxtime_lt_fst_tres  by blast
+  have "conc_stmt_wf slicer"
+    unfolding conc_stmt_wf_def slicer_def by auto
+  moreover have "nonneg_delay_conc slicer"
+    unfolding slicer_def by auto
+  ultimately have "init_sim_valid (\<lambda>tw. fst tw = 0 \<and> wityping \<Gamma> (snd tw)) slicer (\<lambda>tw. (inv tw \<and> wityping \<Gamma> (snd tw)) \<and> inv' tw)"
+    using init_sim_hoare_soundness[OF init_sat_slicer_inv_comb] 
+    by (metis (no_types, lifting) assms(3) conc_wt_cases(1) init_sat_slicer_inv_comb
+    init_sim_hoare_soundness slicer_def strengthen_precondition_init_sim_hoare)
+  hence "inv tw \<and> wityping \<Gamma> (snd tw) \<and> inv' tw"
+    using \<open>init_sim (0, w) slicer tw\<close> fst_conv assms(2) unfolding init_sim_valid_def
+    by (metis snd_conv)
+  hence "inv tw" and "inv' tw" and "wityping \<Gamma> (snd tw)"
+    by auto
+  moreover have "seq_wt \<Gamma> (Bassign_trans OUT (Bslice IN 3 2) 1)"
+    using assms(3) unfolding slicer_def by auto
+  moreover hence "\<Turnstile>\<^sub>s \<lbrace>\<lambda>tw. (inv tw \<and> wityping \<Gamma> (snd tw)) \<and> inv' tw\<rbrace> slicer \<lbrace>inv\<rbrace>"
+    using conc_sim_soundness[OF slicer_conc_sim2'] \<open>conc_stmt_wf slicer\<close> \<open>nonneg_delay_conc slicer\<close>
+    by auto
+  ultimately have "inv tw'"
+    using \<open>tw, i + 1, slicer \<Rightarrow>\<^sub>S tw'\<close> unfolding sim_hoare_valid_def by blast
+  with \<open>i + 1 < fst tw'\<close> show ?thesis
+    unfolding inv_def by auto
+qed
+  
+end
